\documentclass{article}
\usepackage[UTF8]{ctex}
\usepackage{extarrows}
\usepackage{amsmath,amssymb,amsthm,mathtools}
\usepackage [dvipsnames]{xcolor}

\begin{document}
\section{Forward propagation} % (fold)
\label{sec:forward_propagation}

% section forward_propagation (end)
第 \textit{ l }层的正向函数: \\
	cost function:
	\begin{equation}
	J(w,b) = \frac{1}{m} \sum_{i=1}^m L(\hat{y}^{(1) }, y^{(1)})
	\end{equation}

	\begin{equation}
	\begin{split}
	z_{1}^{[i]} &= w_{1}^{[i]}x + b_{1}^{[i]}  ,  a_{1}^{[i]}   = g_{1}^{[i]}(z_{1}^{[i]}) \\
	z_{2}^{[i]} &= w_{2}^{[i]}x + b_{2}^{[i]}  ,  a_{2}^{[i]}   = g_{1}^{[i]}(z_{2}^{[i]}) \\
	z_{3}^{[i]} &= w_{3}^{[i]}x + b_{3}^{[i]}  ,  a_{3}^{[i]}  = g_{3}^{[i]}(z_{3}^{[i]}) \\
	\end{split}
	\end{equation}

	After vectorization:

	\begin{gather}
	\begin{split}
	[z^{[i]}]
	=
	\left[\begin{array}{c}
		 w_{1}^{[i]}  \\  w_{2}^{[i]}  \\  w_{3}^{[i]}
	\end{array}\right]
	X
	+
	\left[\begin{array}{c}
		 b_{1}^{[i]}  \\  b_{2}^{[i]}  \\  b_{3}^{[i]}
	\end{array}\right]
	=
	W^{[i]}X + b^{[i]}
	\end{split}
	\end{gather}
	\begin{gather}
	\begin{split}
	[A^{[i]}]
	=
	\left[\begin{array}{c}
		 g_{1}^{[i]}(z_{1}^{[i]})  \\ g_{2}^{[i]}(z_{1}^{[i]})  \\  g_{3}^{[i]}(z_{1}^{[i]})
	\end{array}\right]
	\end{split}
	\end{gather}

\section{Backward propagation} % (fold)
\label{sec:backward_propagation}
	反向是对 $J(w,b)$，中的 $w , b$进行反向
	\begin{equation}
	\begin{split}
	dz_{1}^{[i]} &= da_{1}^{[i]'}\times g_{1}^{[i]'}(z_{1}^{[i]}) \\
	dz_{2}^{[i]} &= da_{2}^{[i]'}\times g_{2}^{[i]'}(z_{2}^{[i]}) \\
	dz_{3}^{[i]} &= da_{3}^{[i]'}\times g_{3}^{[i]'}(z_{3}^{[i]}) \\
	\end{split}
	\end{equation}

	\begin{gather}
	\begin{split}
	dZ^{[i]} = \sum_{k=1}^m dz_{k}^{[i]} = 
 	dA^{[i]} \times g^{[i]'}(Z^{[i]})
	\end{split}
	\end{gather}

	\begin{equation}
	\begin{split}
	dw_{1}^{[i]} &= dz_{1}^{[i]'}\times a_{1}^{[i-1]} \\
	dw_{2}^{[i]} &= dz_{2}^{[i]'}\times a_{2}^{[i-1]} \\
	dw_{3}^{[i]} &= dz_{3}^{[i]'}\times a_{3}^{[i-1]} \\
	\end{split}
	\end{equation}

	\begin{equation}
	\begin{split}
	dW^{[i]} &= \frac{1}{m}\sum \frac{\partial{J}}{\partial z}\frac{\partial{z}}{\partial w}\\
		& = \frac{1}{m}\sum dz^{[i]}a^{[i-1]}\\
		& = \frac{1}{m}dZ^{[i]}dA^{[i-1]}
	\end{split}
	\end{equation}

	\begin{equation}
	\begin{split}
	db_{1}^{[i]} &= dz_{1}^{[i]} \\
	db_{2}^{[i]} &= dz_{2}^{[i]}  \\
	db_{3}^{[i]} &= dz_{3}^{[i]} \\
	\end{split}
	\end{equation}

	\begin{equation}
	\begin{split}
	db^{[i]} &= \frac{1}{m}\sum \frac{\partial{J}}{\partial z}\frac{\partial{z}}{\partial b}\\
		& = \frac{1}{m}\sum dz^{[i]} \\
		& = \frac{1}{m}np.sum( dZ^{[i]} , axis = 1 , keepdims = True)
	\end{split}
	\end{equation}

	\begin{gather}
	\begin{split}
	[dA^{[i]}]
	=
	\left[\begin{array}{c}
		 g_{1}^{[i]'}(z_{1}^{[i]})  \\ g_{2}^{[i]'}(z_{1}^{[i]})  \\  g_{3}^{[i]'}(z_{1}^{[i]})
	\end{array}\right]
	\end{split}
	\end{gather}
	是对矩阵中的各个元素求导\textbf{注意}

% section backward_propagation (end)
\end{document}